theories/examples/equivalence.v
@@ -1,0 +1,25 @@
+From actris.channel Require Import channel proofmode.
+
+Section equivalence_examples.
+  Context `{heapG Σ, chanG Σ}.
+
+  Lemma binder_swap_equivalence_example :
+    ((<! (x y : Z)> MSG (#x,#y) ; END):iProto Σ)%proto ≡
+    ((<! (y x : Z)> MSG (#x,#y) ; END):iProto Σ)%proto.
+  Proof.
+    apply (uPred.internal_eq_soundness (M:=iResUR Σ)).
+    iApply iProto_message_equiv; [ done | | ].
+    - iIntros "!>" (x y) "_". iExists y, x. eauto.
+    - iIntros "!>" (y x) "_". iExists x, y. eauto.
+  Qed.
+
+  Lemma choice_equivalence_example (P1 P2 Q1 Q2: iProp Σ) (S1 S2 : iProto Σ) :
+    (S1 <{P1 ∗ Q1}+{P2 ∗ Q2}> S2)%proto ≡ (S1 <{Q1 ∗ P1}+{Q2 ∗ P2}> S2)%proto.
+  Proof.
+    apply (uPred.internal_eq_soundness (M:=iResUR Σ)).
+    iApply iProto_choice_equiv; [ done | | | done | done ].
+    iApply prop_ext. iSplit; iIntros "!> [$ $]".
+    iApply prop_ext. iSplit; iIntros "!> [$ $]".
+  Qed.
+
+End equivalence_examples.
